{
 "cells": [
  {
   "cell_type": "markdown",
   "id": "9496bef0-11cb-467b-8793-bfe4cb87dc6e",
   "metadata": {
    "tags": []
   },
   "source": [
    "# Augmented Dickey-Fuller (ADF) Test\n",
    "\n",
    "The Augmented Dickey-Fuller identifies stationarity in an autoregressive process. This is accomplished by testing for the presence</br>\n",
    "of nonstationarity, called the unit root. For example consider the $\\text{AR}(1)$ process,\n",
    "\n",
    "$\n",
    "\\begin{align}\n",
    "X_t = \\varphi X_{t-1} + \\varepsilon_t\n",
    "\\end{align}\n",
    "$\n",
    "\n",
    "where $\\varepsilon_t \\sim \\text{Normal}(0,\\sigma^2)$ and independent. If $\\lvert \\varphi \\rvert < 1$ it can be shown that $X_t$ is stationary. The unit root,</br>\n",
    "$\\lvert \\varphi \\rvert = 1$, is equivalent to brownian motion. \n",
    "\n",
    "### Unit Root Form of $\\text{AR}(1)$\n",
    "\n",
    "The unit root form of $\\text{AR}(1)$ used in the analysis is constructed as follows. Subtracting $X_{t-1}$ from both sides of the expression</br>\n",
    "for $\\text{AR}(1)$ gives,\n",
    "\n",
    "$\n",
    "\\begin{align}\n",
    "X_t - X_{t-1} = \\left( \\varphi - 1\\right) X_{t-1} + \\varepsilon_t\n",
    "\\end{align}\n",
    "$\n",
    "\n",
    "Recall that the lag operator, $L$, is defined by, $L X_t = X_{t-1}, L^2 X_t = X_{t-2}, L^3 X_t = X_{t-3}, \\ldots$. The difference operator is then given by</br> \n",
    "$\\Delta = 1 - L$ and let $\\delta = \\varphi - 1$. It follows that\n",
    "\n",
    "$\n",
    "\\begin{align}\n",
    "& X_t - X_{t-1} = \\left( \\varphi - 1\\right) X_{t-1} + \\varepsilon_t \\\\\n",
    "\\Rightarrow & \\Delta X_t = \\delta X_{t-1} + \\varepsilon_t\n",
    "\\end{align}\n",
    "$\n",
    "\n",
    "Stationarity implies that, $\\delta < 0$, while nonstationarity, unit root, implies $\\delta = 0$. If follows that ADF tests is a lower tail significance test</br>\n",
    "with null hypothesis $\\delta = 0$ and alternative hypothesis $\\delta < 0$. Thus if the test fails $X_t$ is stationary. \n",
    "\n",
    "The lag polynomial is defined by,\n",
    "\n",
    "$\n",
    "\\begin{align}\n",
    "\\Phi^1(L) = 1 - \\varphi L\n",
    "\\end{align}\n",
    "$\n",
    "\n",
    "It follows that,\n",
    "\n",
    "$\n",
    "\\begin{align}\n",
    "\\Phi^1(L)X_t = \\varepsilon_t\n",
    "\\end{align}\n",
    "$\n",
    "\n",
    "The unit root is defined in terms of the lag polynomial by,\n",
    "\n",
    "$\n",
    "\\begin{align}\n",
    "&\\Phi^1(1) =  -\\delta \\\\\n",
    "\\Rightarrow& \\delta = 1 - \\varphi = 0\n",
    "\\end{align}\n",
    "$\n",
    "\n",
    "### Unit Root Form of $\\text{AR}(q)$\n",
    "\n",
    "Following the procedure used for $\\text{AR}(1)$ the unit root form of $\\text{AR}(2)$ can be constructed. The $\\text{AR}(2)$ lag polynomial is given by,\n",
    "\n",
    "$\n",
    "\\begin{align}\n",
    "\\Phi^2(L) = 1 - \\varphi_1 L - \\varphi_2 L^2\n",
    "\\end{align}\n",
    "$\n",
    "\n",
    "If follows that,\n",
    "\n",
    "$\n",
    "\\begin{align}\n",
    "&\\Phi^2(L) X_t = \\varepsilon_t \\\\\n",
    "\\Rightarrow & X_t = \\varphi_1 X_{t-1} + \\varphi_2 X_{t-2} + \\varepsilon_t\n",
    "\\end{align}\n",
    "$\n",
    "\n",
    "To obtain the unit root form subtract $X_{t-1}$ from both sides of $\\text{AR}(2)$ to obtain,\n",
    "\n",
    "$\n",
    "\\begin{align}\n",
    "& X_t - X_{t-1} = \\left( \\varphi_1 - 1 \\right) X_{t-1} + \\varphi_2 X_{t-2} + \\varepsilon_t \\\\\n",
    "\\Rightarrow & \\Delta X_t = \\left( \\varphi_1 - 1 \\right) X_{t-1} + \\varphi_2 X_{t-2} + \\varepsilon_t\n",
    "\\end{align}\n",
    "$\n",
    "\n",
    "Next add and subtract $\\varphi_3 X_{t-1}$ to obtain the final result,\n",
    "\n",
    "$\n",
    "\\begin{align}\n",
    "& \\Delta X_t = \\left( \\varphi_1 - 1 \\right) X_{t-1} + \\varphi_2 X_{t-1} + \\varphi_2 X_{t-2} + \\varepsilon_t - \\varphi_2 X_{t-1} \\\\\n",
    "\\Rightarrow & \\Delta X_t = \\left( \\varphi_2 + \\varphi_1 - 1 \\right) X_{t-1} + \\varphi_2 \\Delta X_{t-1} + \\varepsilon_t\n",
    "\\end{align}\n",
    "$\n",
    "\n",
    "Let $\\delta = \\varphi_2 + \\varphi_1 - 1$ to obtain the unit root form,\n",
    "\n",
    "$\n",
    "\\begin{align}\n",
    "\\Delta X_t = \\delta X_{t-1} + \\varphi_2 \\Delta X_{t-1} + \\varepsilon_t\n",
    "\\end{align}\n",
    "$\n",
    "\n",
    "The unit root is defined in terms of the lag polynomial by,\n",
    "\n",
    "$\n",
    "\\begin{align}\n",
    "&\\Phi^2(1) = -\\delta \\\\\n",
    "\\Rightarrow& \\delta = 1 - \\varphi_1 - \\varphi_2 = 0\n",
    "\\end{align}\n",
    "$\n",
    "\n",
    "This procedure can be repeated for autoregressive processes of arbitrary order. $\\text{AR}(q)$ is defined by\n",
    "\n",
    "$\n",
    "\\begin{align}\n",
    "&\\Phi^q(L) = 1 - \\varphi_1 L + \\varphi_2 L^2 - \\cdots - \\varphi_q L^q \\\\\n",
    "\\Rightarrow & \\Phi^q(L) X_t = \\varepsilon_t \\\\\n",
    "\\Rightarrow & X_t = \\varphi_1 X_{t-1} + \\varphi_2 X_{t-2} + \\cdots + + \\varphi_q X_{t-q} + \\varepsilon_t\n",
    "\\end{align}\n",
    "$\n",
    "\n",
    "the unit root form is given by,\n",
    "\n",
    "$\n",
    "\\begin{align}\n",
    "\\Delta X_t = \\delta X_{t-1} + C_1 \\Delta X_{t-1} + C_2 \\Delta X_{t-2} + \\cdots + C_{q-1} \\Delta X_{t- \\left( q - 1 \\right)} + \\varepsilon_t\n",
    "\\end{align}\n",
    "$\n",
    "\n",
    "where,\n",
    "\n",
    "$\n",
    "\\begin{align}\n",
    "&\\delta = \\varphi_1 + \\varphi_2 + \\cdots + \\varphi_q \\\\\n",
    "&\\Phi^q(1) = -\\delta \\\\\n",
    "&C_i = -\\sum_{j=i+1}^q \\varphi_j\n",
    "\\end{align}\n",
    "$\n",
    "\n",
    "### $\\text{AR}(1)$ Test Statistic\n",
    "\n",
    "The OLS estimate for the $\\text{AR}(1)$ coefficient $\\varphi$  is given by,\n",
    "\n",
    "$\n",
    "\\begin{align}\n",
    "\\hat{\\varphi} = \\frac{\\sum_{t=1}^T X_t X_{t-1}}{\\sum_{t=1}^T X^2_{t-1}}\n",
    "\\end{align}\n",
    "$\n",
    "\n",
    "Using $X_t = \\Delta X_t + X_{t-1}$ and $\\hat{\\delta} = \\hat{\\varphi} - 1$ gives,\n",
    "\n",
    "$\n",
    "\\begin{align}\n",
    "\\hat{\\delta} = \\frac{\\sum_{t=1}^T X_{t-1} \\varepsilon_t}{\\sum_{t=1}^T X^2_{t-1}}\n",
    "\\end{align}\n",
    "$\n",
    "\n",
    "From this expression it can be shown that,\n",
    "\n",
    "$\n",
    "\\begin{align}\n",
    "&\\text{E}(\\hat{\\delta}) = 0 \\\\\n",
    "&\\text{Var}(\\hat{\\delta}) = \\frac{\\sigma}{\\sum_{t=1}^T X^2_{t-1}}\n",
    "\\end{align}\n",
    "$\n",
    "\n",
    "The test statistic is given by,\n",
    "\n",
    "$\n",
    "\\begin{align}\n",
    "t = \\frac{\\hat{\\delta}}{\\sqrt{\\text{Var}({\\hat{\\delta}})}}\n",
    "\\end{align}\n",
    "$\n",
    "\n",
    "The distribution of $t$ is not a standard distribution but has a stochastic integral representation that must be evaluated numerically, namely,\n",
    "\n",
    "$\n",
    "\\begin{align}\n",
    "T \\hat{\\delta} \\sim \\frac{\\int_0^1 B(s) dB(s)}{\\int_0^1 B^2(s) ds}\n",
    "\\end{align}\n",
    "$\n",
    "\n",
    "The numerator integral can be evaluated to obtain,\n",
    "\n",
    "$\n",
    "\\begin{align}\n",
    "\\int_0^1 B(s) dB(s) = \\frac{1}{2} \\left[ B^2(1) - 1 \\right]\n",
    "\\end{align}\n",
    "$\n",
    "\n",
    "The final result is given by,\n",
    "\n",
    "$\n",
    "\\begin{align}\n",
    "T \\hat{\\delta} \\sim \\frac{\\frac{1}{2} \\left[ B^2(1) - 1 \\right]}{\\int_0^1 B^2(s) ds}\n",
    "\\end{align}\n",
    "$\n"
   ]
  },
  {
   "cell_type": "code",
   "execution_count": null,
   "id": "fd7d8827-5c1b-4fea-b5af-50cf78c31e60",
   "metadata": {},
   "outputs": [],
   "source": []
  }
 ],
 "metadata": {
  "kernelspec": {
   "display_name": "Python 3 (ipykernel)",
   "language": "python",
   "name": "python3"
  },
  "language_info": {
   "codemirror_mode": {
    "name": "ipython",
    "version": 3
   },
   "file_extension": ".py",
   "mimetype": "text/x-python",
   "name": "python",
   "nbconvert_exporter": "python",
   "pygments_lexer": "ipython3",
   "version": "3.9.2"
  }
 },
 "nbformat": 4,
 "nbformat_minor": 5
}
